moving stuff from Infer

src/Infer.v
@@ -20,21 +20,6 @@ Require Import SimpleTypes.
 Require Import Subst.
 Require Import MyLtacs.
 
-Fixpoint compute_generic_subst (st : id) (n : nat) : list ty  * id:=
-  match n with
-  | 0 => (nil, st)
-  | S n' =>
-    match compute_generic_subst (S st) n' with
-    | (l', st') => (var st :: l', st')
-    end
-  end.
-
-Fixpoint compute_subst (i : id) (l : list ty) : substitution :=
-  match l return substitution with
-  | nil => nil
-  | t :: l' => (i, t) :: compute_subst (S i) l'
-  end.
-
 Inductive SubstFailure :  Prop :=
 | substFail : SubstFailure.
 
@@ -90,63 +75,6 @@ Program Definition look_dep (x : id) (G : ctx) :
   | None => failT (MissingVar' x (missingVar x)) schm
   end.
 
-Lemma assoc_subst_exists : forall (G : ctx) (i : id) (s : substitution) (sigma : schm),
-    in_ctx i (apply_subst_ctx s G) = Some sigma ->
-    {sigma' : schm | in_ctx i G = Some sigma' /\ sigma = apply_subst_schm s sigma'}.
-Proof.
-  refine (fix assoc_subst_exists G i s sigma :
-            in_ctx i (apply_subst_ctx s G) = Some sigma ->
-            {sigma' : schm | in_ctx i G = Some sigma' /\ sigma = apply_subst_schm s sigma'} :=
-            (fun PP => match G as G0 return G = G0 -> {sigma' : schm | in_ctx i G = Some sigma' /\ sigma = apply_subst_schm s sigma'} with
-            | nil => fun L => exist _ _ _
-            | ((j, sigma')::G') => fun L =>  if (eq_id_dec i j) then exist _ sigma' _ else
-                                       match assoc_subst_exists G' i s sigma _ with
-                                       | exist _ sigma'' _ => exist _ sigma'' _
-                                       end
-                    end _)  );
-  crush.
-  Unshelve. auto.
-Qed.
-
-Hint Resolve assoc_subst_exists.
-
-Lemma apply_subst_app : forall (s1 s2 : substitution) (st : id),
-    find_subst s1 st = None -> apply_subst (s1 ++ s2) (var st) = apply_subst s2 (var st).
-Proof.
-  induction s1;
-  crush.
-Qed.
-
-Hint Resolve apply_subst_app.
-Hint Rewrite apply_subst_app:RE.
-
-Lemma not_in_domain_compute : forall (is_s : inst_subst) (st0 st1 : id),
-    st0 < st1 -> find_subst (compute_subst st1 is_s) st0 = None.
-Proof.
-  induction is_s; crush.
-Qed.
-
-Hint Resolve not_in_domain_compute.
-Hint Rewrite not_in_domain_compute:RE.
-
-Lemma apply_app_compute_subst : forall (is_s : inst_subst) (s : substitution) (st0 st1 : id),
-       st0 < st1 -> apply_subst ((compute_subst st1 is_s) ++ s) (var st0) = apply_subst s (var st0).
-Proof.
-  induction is_s;
-  crush.
-Qed.
-
-Hint Resolve apply_app_compute_subst.
-Hint Rewrite apply_app_compute_subst:RE.
-
-Lemma apply_subst_inst_to_ty_to_schm : forall (is_s : inst_subst) (tau : ty),
-    apply_inst_subst is_s (ty_to_schm tau) = Some_schm tau.
-Proof.
-  induction tau; crush.
-Qed.
-
-Hint Resolve apply_subst_inst_to_ty_to_schm.
-Hint Rewrite apply_subst_inst_to_ty_to_schm:RE.
 
 Lemma assoc_stamp_in_subst_app2 : forall (s1 s2 : substitution) (st : id) (tau : ty),
  find_subst s1 st = Some tau -> find_subst (s1 ++ s2) st = Some tau.
@@ -157,102 +85,11 @@ Qed.
 Hint Resolve assoc_stamp_in_subst_app2.
 Hint Rewrite assoc_stamp_in_subst_app2:RE.
 
-Lemma apply_app : forall (s1 s2 : substitution) (st : id) (tau : ty),
-    find_subst s1 st = Some tau -> apply_subst (s1 ++ s2) (var st) = tau.
-Proof.
-  induction s1; crush.
-Qed.
-
-Hint Resolve apply_app.
-Hint Rewrite apply_app:RE.
-
-Lemma compute_subst_cons_rwt : forall (st : id) (tau : ty) (sg : inst_subst),
-    compute_subst st (tau :: sg) = (st, tau) :: compute_subst (S st) sg.
-auto.
-Qed.
-
-Hint Resolve compute_subst_cons_rwt.
-Hint Rewrite compute_subst_cons_rwt:RE.
-
-Lemma find_subst_id_compute : forall (i : id) (is_s : inst_subst) (st : id) (tau : ty),
-    nth_error is_s i = Some tau -> find_subst (compute_subst st is_s) ((st + i)) = Some tau.
-Proof.
-  induction i; crush.
-  destruct is_s; crush.
-  destruct is_s. crush.
-  rewrite compute_subst_cons_rwt.
-  crush.
-  rewrite <- Nat.add_succ_comm.
-  erewrite IHi; eauto.
-Qed.
-
-Hint Resolve find_subst_id_compute.
-Hint Rewrite find_subst_id_compute:RE.
-
-Lemma t_is_app_T_aux : forall (sigma : schm) (tau tau' : ty) (s : substitution) (p : nat) (st : id) (x : list ty),
-    new_tv_schm sigma st -> max_gen_vars sigma <= p ->
-    apply_inst_subst (compute_inst_subst st p) sigma = Some_schm tau ->
-    apply_inst_subst x (apply_subst_schm s sigma) = Some_schm tau' ->
-    tau' = apply_subst ((compute_subst st x) ++ s) tau.
-Proof.
-  induction sigma.
-  - intros.
-    inversion H. subst.
-    simpl in H1. inversion H1.
-    simpl in H2. fold (apply_subst s (var i)) in H2.
-    rewrite apply_subst_inst_to_ty_to_schm in H2.
-    inversion H2.
-    rewrite apply_app_compute_subst; eauto.
-   - crush. 
-   - intros. 
-     simpl in *.
-     rewrite nth_error_compute_inst_Some in *; eauto.
-     inversion H1. inversion H. subst.
-     cases (nth_error x i).
-     inversion H2. subst. clear H2 H1.
-     erewrite apply_app; eauto.
-     rewrite Nat.add_comm.
-     eapply find_subst_id_compute; eauto.
-     inversion H2.
-   - intros. 
-     inversion H. subst.
-     simpl in H0. rewrite apply_subst_schm_arrow in H2.
-     edestruct (exist_arrow_apply_inst_arrow (compute_inst_subst st p)); eauto.
-     destruct H3.
-     edestruct (exist_arrow_apply_inst_arrow x); eauto.
-     destruct H4. subst.
-     apply and_arrow_apply_inst_arrow in H1.
-     destruct H1.
-     apply and_arrow_apply_inst_arrow in H2.
-     destruct H2.
-     simpl.
-     eapply Nat.max_lub_r in H0 as H0r.
-     eapply Nat.max_lub_l in H0 as H0l.
-     erewrite <- IHsigma1; eauto.
-     erewrite <- IHsigma2; eauto.
-Qed.
-
-Hint Resolve t_is_app_T_aux.
-
 Definition completeness (e : term) (G : ctx) (tau : ty) (s : substitution) (st : id) :=
   forall (tau' : ty) (phi : substitution),
     has_type (apply_subst_ctx phi G) e tau' -> 
     exists s', tau' = apply_subst s' tau /\
     (forall x : id, x < st -> apply_subst phi (var x) = apply_subst s' (apply_subst s (var x))).
-
-Lemma apply_subst_app1 : forall (s1 s2 : substitution) (st : id),
- find_subst s1 st = None -> apply_subst (compose_subst s1 s2) (var st) = apply_subst s2 (var st).
-Proof.
-  intros.
-  induction s1.
-  - mysimp.
-  - simpl in *.
-    destruct a.
-    mysimp.
-Qed.
-
-Hint Resolve apply_subst_app1.
-Hint Rewrite apply_subst_app1 : subst.
 
 (** Gives you a fresh variable *)
 Program Definition fresh : @Infer (@top id) id (fun i x f => S i = f /\ i = x) := fun n => exist _ (inleft (n, S n)) _.
@@ -285,64 +122,6 @@ Next Obligation.
   eauto.
 Defined.
     
-Lemma add_subst_rewrite_for_modified_stamp : forall (s : substitution) (i : id) (tau : ty),
-    (apply_subst ((i, tau)::s) (var i)) = tau.
-  intros.
-  mysimp.
-Qed.
-
-Hint Resolve add_subst_rewrite_for_modified_stamp.
-
-Lemma add_subst_rewrite_for_unmodified_stamp : forall (s : substitution) (i j : id) (tau : ty),
-    i <> j -> (apply_subst ((i, tau):: s)) (var j) = apply_subst s (var j).
-  intros; induction s; mysimp.
-Qed.
-
-Hint Resolve add_subst_rewrite_for_unmodified_stamp.
-
-Lemma img_ids_append_cons : forall a t s, img_ids ((a, t)::s) = ids_ty t ++ img_ids s.
-Proof.
-  induction t; mysimp.
-Qed.
-
-Lemma new_tv_subst_false : forall st s t, new_tv_subst ((st, t) :: s) st -> False.
-Proof.
-  intros.
-  induction s. inversion H.
-  specialize H0 with (x:=st).
-  simpl in H0.
-  destruct (eq_id_dec st st);
-  intuition.
-  inversion H.
-  simpl in H0.
-  specialize H0 with (x:=st).
-  destruct (eq_id_dec st st); intuition.
-Qed.
-
-Hint Resolve new_tv_subst_false.
-
-Lemma new_tv_subst_cons_diff : forall a st t s, a <> st -> new_tv_subst ((a, t) :: s) st -> new_tv_subst s st.
-Proof.
-  intros.
-  econstructor.
-  intros.
-  unfold FV_subst in H1.
-  inversion H0.
-  eapply H2.
-  simpl.
-  destruct (eq_id_dec a x); try contradiction; auto.
-  apply in_list_id_or_append_inversion in H1.
-  destruct H1.
-  apply in_list_id_append1; auto.
-  apply in_list_id_append2.
-  simpl.
-  rewrite img_ids_append_cons.
-  apply in_list_id_append2.
-  assumption.
-Qed.
-
-Hint Resolve new_tv_subst_cons_diff.
-
 Unset Implicit Arguments.
 
 Program Fixpoint W_hoare (e : term) (G : ctx) {struct e} :
@@ -405,7 +184,7 @@ Next Obligation.  (* Case: postcondition of var *)
     subst.
     inversion H7.
     rename x into is_s.
-    destruct (assoc_subst_exists G st0 phi sigma H5) as [sigma' H5'].
+    destruct (@assoc_subst_exists G st0 phi sigma H5) as [sigma' H5'].
     destruct H5' as [H51  H52].
     destruct H7.
     exists ((compute_subst st1 is_s) ++ phi).
